verified/Seq.dfy
@@ -15,3 +15,23 @@ function {:opaque} SeqRepeat<T>(count:nat, elt:T) : seq<T>
 {
     if count == 0 then [] else [elt] + SeqRepeat<T>(count - 1, elt)
 }
+
+function {:opaque} MapSeqToSeq<T,U>(s:seq<T>, func:T->U) : seq<U>
+    reads func.reads;
+    requires forall i :: func.reads(i) == {};
+    requires forall i :: 0 <= i < |s| ==> func.requires(s[i]);
+    ensures |MapSeqToSeq(s, func)| == |s|;
+    ensures forall i {:trigger func(s[i])} {:trigger MapSeqToSeq(s,func)[i]} :: 0 <= i < |s| ==> func(s[i]) == MapSeqToSeq(s,func)[i];
+{
+    if |s| == 0 then []
+    else [func(s[0])] + MapSeqToSeq(s[1..], func)
+}
+
+function {:opaque} IMapSeqToSeq<T,U>(s:seq<T>, func:imap<T,U>) : seq<U>
+    requires forall i :: 0 <= i < |s| ==> s[i] in func;
+    ensures |IMapSeqToSeq(s, func)| == |s|;
+    ensures forall i {:trigger func[s[i]]} {:trigger IMapSeqToSeq(s,func)[i]} :: 0 <= i < |s| ==> func[s[i]] == IMapSeqToSeq(s,func)[i];
+{
+    if |s| == 0 then []
+    else [func[s[0]]] + IMapSeqToSeq(s[1..], func)
+}
