verified/ptables.i.dfy
@@ -1,0 +1,170 @@
+include "pagedb.i.dfy"
+include "entry.s.dfy"
+
+lemma UserExecutionMemInvariant(s:state, s':state, d:PageDb, l1:PageNr)
+    requires ValidState(s) && SaneMem(s.m)
+    requires evalUserspaceExecution(s, s')
+    requires validPageDb(d)
+    requires pageDbCorresponds(s.m, d)
+    requires nonStoppedL1(d, l1)
+    requires s.conf.ttbr0.ptbase == page_paddr(l1)
+    ensures WSMemInvariantExceptAddrspaceAtPage(s, s', d, l1)
+{
+    var l1pg := extractPage(s.m, l1);
+    var e := d[l1].entry;
+    assert e.L1PTable? && wellFormedPageDbEntryTyped(e);
+    assert pageContentsCorresponds(l1, d[l1], l1pg);
+    reveal_pageContentsCorresponds();
+    assert pageDbL1PTableCorresponds(l1, e, l1pg);
+    assume false;
+}
+
+function mkAbsPTE(pte: L2PTE): Maybe<AbsPTE>
+    requires PhysBase() == KOM_DIRECTMAP_VBASE()
+    ensures var r := mkAbsPTE(pte); r.Just? ==> WellformedAbsPTE(r.v)
+{
+    match pte {
+        case SecureMapping(p, w, x) => Just(
+            var pa := page_paddr(p);
+            assert PageAligned(pa) && isUInt32(pa + PhysBase());
+            AbsPTE(pa, w, x))
+        case InsecureMapping(p, w) => Just(
+            assert validInsecurePageNr(p);
+            var pa := p * PAGESIZE();
+            assert 0 <= pa < KOM_PHYSMEM_LIMIT();
+            assert PageAligned(pa) && isUInt32(pa + PhysBase());
+            AbsPTE(pa, w, false))
+        case NoMapping => Nothing
+    }
+}
+
+lemma {:axiom} l2ptesmatch(pte: L2PTE)
+    requires PhysBase() == KOM_DIRECTMAP_VBASE()
+    ensures ExtractAbsL2PTE(mkL2Pte(pte)) == Just(mkAbsPTE(pte))
+/* FIXME: this is really gross right now (and contains several
+ * assumes!), largely due to problems in Boogie/Dafny's bitvector
+ * support. It's also hopelessly unstable.
+{
+    var pteword := mkL2Pte(pte);
+    var ptebv := IntAsBits(pteword);
+    var extracted := ExtractAbsL2PTE(pteword);
+    if pte.NoMapping? {
+        assert ptebv == 0;
+        assert extracted == Just(Nothing) by {reveal_BitAnd();}
+    } else {
+        var pa, w, x;
+        match pte {
+            case SecureMapping(p, ws, xs) =>
+                pa, w, x := page_paddr(p), ws, xs;
+            case InsecureMapping(p, wi) =>
+                pa, w, x := p * PAGESIZE(), wi, false;
+        }
+        assert pteword == ARM_L2PTE(pa, w, x);
+        var pabv := IntAsBits(pa);
+        assert PAGESIZE() == 0x1000 == pow2(12) by { reveal_pow2(); }
+        assert pa % PAGESIZE() == 0;
+        assert BitmaskLow(12) == 0xfff by { reveal_BitmaskLow(); assume 1 as bv32 << 12 == 0x1000; }
+        reveal_BitAnd();
+        assert BitAnd(pabv, 0xfff) == 0 by { lemma_Bitmask(pabv, 12); lemma_BitModEquiv(pabv, 0x1000); }
+        var nxbit:bv32 := if x then 0 else ARM_L2PTE_NX_BIT();
+        var robit:bv32 := if w then 0 else ARM_L2PTE_RO_BIT();
+        assert ARM_L2PTE_NX_BIT() == 1 && ARM_L2PTE_RO_BIT() == 0x200;
+        assert ptebv == pabv | ARM_L2PTE_CONST_BITS() | 0x2 | nxbit | robit;
+        assert BitAnd(ptebv, 0x3) == 2;
+        assert BitAnd(ptebv, 0xfdfc) == ARM_L2PTE_CONST_BITS();
+        assert BitAnd(ptebv, 0xfffff000) == IntAsBits(pa);
+        assert pa == BitwiseMaskHigh(pteword, 12) by { reveal_BitmaskHigh(); reveal_BitNot(); assume 1 as bv32 << 12 == 0x1000; }
+        assert ptebv & ARM_L2PTE_NX_BIT() == nxbit;
+        assert ptebv & ARM_L2PTE_RO_BIT() == robit;
+        assert isUInt32(pa + PhysBase());
+        assert extracted == Just(mkAbsPTE(pte));
+    }
+} */
+
+function getAbsPTE(d:PageDb, l2:PageNr, i:int, j:int): Maybe<AbsPTE>
+    requires validPageDb(d)
+    requires validL2PTPage(d, l2) && !hasStoppedAddrspace(d, l2)
+    requires 0 <= i < 4 && 0 <= j < ARM_L2PTES()
+    requires PhysBase() == KOM_DIRECTMAP_VBASE()
+    ensures var r := getAbsPTE(d, l2, i, j); r.Just? ==> WellformedAbsPTE(r.v)
+{
+    mkAbsPTE(d[l2].entry.l2pt[i * 4 + j])
+}
+
+lemma lemma_memstatecontainspage(s:memstate, p:PageNr)
+    requires SaneMem(s)
+    ensures memContainsPage(s.addresses, p)
+{
+    var va := page_monvaddr(p);
+    assert ValidMemRange(va, va + PAGESIZE());
+    reveal_ValidMemState();
+}
+
+predicate l2tablesmatch(s:memstate, p:PageNr, e:PageDbEntryTyped)
+    requires PhysBase() == KOM_DIRECTMAP_VBASE()
+    requires ValidMemState(s)
+    requires e.L2PTable? && wellFormedPageDbEntryTyped(e)
+{
+    var vbase := page_monvaddr(p);
+    ValidMemRange(vbase, vbase + PAGESIZE())
+    && forall i | 0 <= i < 4 :: ExtractAbsL2PTable(s, vbase + i * ARM_L2PTABLE_BYTES(), 0)
+        == Just(mkAbsL2PTable(e, i))
+}
+
+lemma lemma_l2tablesmatch(s:memstate, p:PageNr, e:PageDbEntryTyped)
+    requires SaneMem(s)
+    requires PhysBase() == KOM_DIRECTMAP_VBASE()
+    requires e.L2PTable? && wellFormedPageDbEntryTyped(e)
+    requires pageDbL2PTableCorresponds(p, e, extractPage(s, p))
+    ensures l2tablesmatch(s, p, e)
+{
+    lemma_memstatecontainspage(s, p);
+    assume false; // TODO
+}
+
+function mkAbsL2PTable(e:PageDbEntryTyped, i:int): AbsL2PTable
+    requires PhysBase() == KOM_DIRECTMAP_VBASE()
+    requires e.L2PTable? && wellFormedPageDbEntryTyped(e)
+    requires 0 <= i < 4
+    ensures WellformedAbsL2PTable(mkAbsL2PTable(e, i))
+{
+    var l2ptes := e.l2pt[i*ARM_L2PTES()..(i+1)*ARM_L2PTES()];
+    var res := MapSeqToSeq(l2ptes, mkAbsPTE);
+    assert |res| == ARM_L2PTES();
+    res
+}
+
+function mkAbsPTable'(d:PageDb, l1:PageNr, idx:int): AbsPTable
+    requires PhysBase() == KOM_DIRECTMAP_VBASE()
+    requires validPageDb(d)
+    requires nonStoppedL1(d, l1)
+    requires 0 <= idx <= NR_L1PTES()
+    decreases NR_L1PTES() - idx
+    ensures var r := mkAbsPTable'(d, l1, idx);
+        |r| == (NR_L1PTES() - idx) * 4
+        && forall i :: 0 <= i < |r| && r[i].Just? ==> WellformedAbsL2PTable(fromJust(r[i]))
+{
+    if idx == NR_L1PTES() then [] else
+        var l2e := d[l1].entry.l1pt[idx];
+        var first :=
+            if l2e.Nothing?
+            then [Nothing, Nothing, Nothing, Nothing]
+            else
+                assert validL1PTable(d, l1) by { reveal_validPageDb(); }
+                var e' := d[fromJust(l2e)];
+                assert e'.PageDbEntryTyped?;
+                var e := e'.entry;
+                assert e.L2PTable? && wellFormedPageDbEntryTyped(e);
+                [Just(mkAbsL2PTable(e, 0)), Just(mkAbsL2PTable(e, 1)),
+                 Just(mkAbsL2PTable(e, 2)), Just(mkAbsL2PTable(e, 3))];
+        first + mkAbsPTable'(d, l1, idx + 1)
+}
+
+function mkAbsPTable(d:PageDb, l1:PageNr): AbsPTable
+    requires PhysBase() == KOM_DIRECTMAP_VBASE()
+    requires validPageDb(d)
+    requires nonStoppedL1(d, l1)
+    ensures WellformedAbsPTable(mkAbsPTable(d, l1))
+{
+    mkAbsPTable'(d, l1, 0)
+}
